Slew of theorems about RC and RTC (new constants).

src/relation/relationScript.sml
@@ -10,25 +10,40 @@ struct
 
 
 open HolKernel Parse boolLib QLib tautLib mesonLib Rsyntax;
+open simpLib boolSimps
 infix ORELSE ORELSEC THEN THENL |->;
 
 val _ = new_theory "relation";
 
 
-val TC_DEF = 
+val TC_DEF =
 Q.new_definition
 ("TC_DEF",
-  `TC (R:'a->'a->bool) a b = 
-    !P. 
+  `TC (R:'a->'a->bool) a b =
+    !P.
        (!x y. R x y ==> P x y) /\
        (!x y z. P x y /\ P y z ==> P x z)
        ==> P a b`);
 
+val RTC_DEF = new_definition(
+  "RTC_DEF",
+  ``RTC (R : 'a -> 'a -> bool) a b =
+      !P.  (!x. P x x) /\
+           (!x y z. R x y /\ P y z ==> P x z) ==>
+           P a b``);
 
-val transitive_def = 
+val RC_DEF = new_definition(
+  "RC_def",
+  ``RC (R:'a->'a->bool) x y = (x = y) \/ R x y``);
+
+val transitive_def =
 Q.new_definition
-("transitive_def", 
+("transitive_def",
    `transitive (R:'a->'a->bool) = !x y z. R x y /\ R y z ==> R x z`);
+
+val reflexive_def = new_definition(
+  "reflexive_def",
+  ``reflexive (R:'a->'a->bool) = !x. R x x``);
 
 
 val TC_TRANSITIVE = Q.store_thm("TC_TRANSITIVE",
@@ -37,19 +52,81 @@ REWRITE_TAC[transitive_def,TC_DEF]
  THEN REPEAT STRIP_TAC
  THEN RES_TAC THEN ASM_MESON_TAC[]);
 
+val RTC_INDUCT = store_thm(
+  "RTC_INDUCT",
+  ``!R P. (!x. P x x) /\ (!x y z. R x y /\ P y z ==> P x z) ==>
+          (!x (y:'a). RTC R x y ==> P x y)``,
+  REWRITE_TAC [RTC_DEF] THEN MESON_TAC []);
+
+val TC_RULES = store_thm(
+  "TC_RULES",
+  ``!R. (!x (y:'a). R x y ==> TC R x y) /\
+        (!x y z. TC R x y /\ TC R y z ==> TC R x z)``,
+  REWRITE_TAC [TC_DEF] THEN REPEAT STRIP_TAC THENL [
+    ASM_MESON_TAC [],
+    FIRST_ASSUM MATCH_MP_TAC THEN RES_TAC THEN ASM_MESON_TAC []
+  ]);
+
+val RTC_RULES = store_thm(
+  "RTC_RULES",
+  ``!R. (!x. RTC R (x:'a) x) /\ (!x y z. R x y /\ RTC R y z ==> RTC R x z)``,
+  SIMP_TAC bool_ss [RTC_DEF] THEN MESON_TAC []);
+
+val RTC_STRONG_INDUCT = store_thm(
+  "RTC_STRONG_INDUCT",
+  ``!R P. (!x. P x x) /\ (!x y z. R x y /\ RTC R y z /\ P y z ==> P x z) ==>
+          (!x (y:'a). RTC R x y ==> P x y)``,
+  REPEAT GEN_TAC THEN STRIP_TAC THEN
+  MATCH_MP_TAC ((CONV_RULE (SIMP_CONV bool_ss [RTC_RULES]) o
+                 Q.SPECL [`R`, `\u v. RTC R u v /\ P u v`]) RTC_INDUCT) THEN
+  REPEAT STRIP_TAC THEN ASM_MESON_TAC [RTC_RULES]);
+
+val RTC_RTC = store_thm(
+  "RTC_RTC",
+  ``!R (x:'a) y. RTC R x y ==> !z. RTC R y z ==> RTC R x z``,
+  GEN_TAC THEN HO_MATCH_MP_TAC RTC_STRONG_INDUCT THEN MESON_TAC [RTC_RULES]);
+
+val RTC_TRANSITIVE = store_thm(
+  "RTC_TRANSITIVE",
+  ``!R:'a->'a->bool. transitive (RTC R)``,
+  REWRITE_TAC [transitive_def] THEN MESON_TAC [RTC_RTC]);
+
+val RTC_REFLEXIVE = store_thm(
+  "RTC_REFLEXIVE",
+  ``!R:'a->'a->bool. reflexive (RTC R)``,
+  MESON_TAC [reflexive_def, RTC_RULES]);
+
+val RC_REFLEXIVE = store_thm(
+  "RC_REFLEXIVE",
+  ``!R:'a->'a->bool. reflexive (RC R)``,
+  MESON_TAC [reflexive_def, RC_DEF]);
 
 val TC_SUBSET = Q.store_thm("TC_SUBSET",
 `!R x (y:'a). R x y ==> TC R x y`,
 REWRITE_TAC[TC_DEF] THEN MESON_TAC[]);
 
+val RTC_SUBSET = store_thm(
+  "RTC_SUBSET",
+  ``!R (x:'a) y. R x y ==> RTC R x y``,
+  MESON_TAC [RTC_RULES]);
+
+val RC_SUBSET = store_thm(
+  "RC_SUBSET",
+  ``!R (x:'a) y. R x y ==> RC R x y``,
+  MESON_TAC [RC_DEF]);
+
+val RC_RTC = store_thm(
+  "RC_RTC",
+  ``!R (x:'a) y. RC R x y ==> RTC R x y``,
+  MESON_TAC [RC_DEF, RTC_RULES]);
+
 
 val TC_INDUCT = Q.store_thm("TC_INDUCT",
 `!(R:'a->'a->bool) P.
-   (!x y. R x y ==> P x y) /\ 
+   (!x y. R x y ==> P x y) /\
    (!x y z. P x y /\ P y z ==> P x z)
    ==> !u v. (TC R) u v ==> P u v`,
 REWRITE_TAC[TC_DEF] THEN MESON_TAC[]);
-
 
 val TC_INDUCT_TAC =
  let val tc_thm = TC_INDUCT
@@ -66,26 +143,108 @@ val TC_INDUCT_TAC =
       in MATCH_MP_TAC tc_thm' (asl,w)
       end
       handle _ => raise HOL_ERR{origin_structure = "<top-level>",
-                     origin_function = "TC_INDUCT_TAC", 
+                     origin_function = "TC_INDUCT_TAC",
                      message = "Unanticipated term structure"}
  in tac
  end;
 
 
-val TC_CASES1 = 
+val TC_RTC = store_thm(
+  "TC_RTC",
+  ``!R (x:'a) y. TC R x y ==> RTC R x y``,
+  GEN_TAC THEN TC_INDUCT_TAC THEN MESON_TAC [RTC_RULES, RTC_RTC]);
+
+val RTC_TC_RC = store_thm(
+  "RTC_TC_RC",
+  ``!R (x:'a) y. RTC R x y ==> RC R x y \/ TC R x y``,
+  GEN_TAC THEN HO_MATCH_MP_TAC RTC_STRONG_INDUCT THEN
+  REPEAT STRIP_TAC THENL [
+    REWRITE_TAC [RC_DEF],
+    FULL_SIMP_TAC bool_ss [RC_DEF] THEN ASM_MESON_TAC [TC_RULES],
+    ASM_MESON_TAC [TC_RULES]
+  ]);
+
+val TC_RC_EQNS = store_thm(
+  "TC_RC_EQNS",
+  ``!R:'a->'a->bool. (RC (TC R) = RTC R) /\ (TC (RC R) = RTC R)``,
+  REPEAT STRIP_TAC THEN
+  CONV_TAC (Q.X_FUN_EQ_CONV `u`) THEN GEN_TAC THEN
+  CONV_TAC (Q.X_FUN_EQ_CONV `v`) THEN GEN_TAC THEN
+  EQ_TAC THENL [
+    REWRITE_TAC [RC_DEF] THEN MESON_TAC [TC_RTC, RTC_RULES],
+    Q.ID_SPEC_TAC `v` THEN Q.ID_SPEC_TAC `u` THEN
+    HO_MATCH_MP_TAC RTC_STRONG_INDUCT THEN
+    SIMP_TAC bool_ss [RC_DEF] THEN MESON_TAC [TC_RULES],
+    Q.ID_SPEC_TAC `v` THEN Q.ID_SPEC_TAC `u` THEN
+    HO_MATCH_MP_TAC TC_INDUCT THEN MESON_TAC [RC_RTC, RTC_RTC],
+    Q.ID_SPEC_TAC `v` THEN Q.ID_SPEC_TAC `u` THEN
+    HO_MATCH_MP_TAC RTC_INDUCT THEN MESON_TAC [TC_RULES, RC_DEF]
+  ]);
+
+val RC_IDEM = store_thm(
+  "RC_IDEM",
+  ``!R:'a->'a->bool.  RC (RC R) = RC R``,
+  GEN_TAC THEN
+  CONV_TAC (Q.X_FUN_EQ_CONV `u`) THEN GEN_TAC THEN
+  CONV_TAC (Q.X_FUN_EQ_CONV `v`) THEN GEN_TAC THEN
+  SIMP_TAC bool_ss [RC_DEF] THEN MESON_TAC []);
+
+val TC_IDEM = store_thm(
+  "TC_IDEM",
+  ``!R:'a->'a->bool.  TC (TC R) = TC R``,
+  GEN_TAC THEN
+  CONV_TAC (Q.X_FUN_EQ_CONV `u`) THEN GEN_TAC THEN
+  CONV_TAC (Q.X_FUN_EQ_CONV `v`) THEN GEN_TAC THEN
+  EQ_TAC THEN Q.ID_SPEC_TAC `v` THEN Q.ID_SPEC_TAC `u` THEN
+  HO_MATCH_MP_TAC TC_INDUCT THEN MESON_TAC [TC_RULES]);
+
+val RTC_IDEM = store_thm(
+  "RTC_IDEM",
+  ``!R:'a->'a->bool.  RTC (RTC R) = RTC R``,
+  GEN_TAC THEN
+  CONV_TAC (Q.X_FUN_EQ_CONV `u`) THEN GEN_TAC THEN
+  CONV_TAC (Q.X_FUN_EQ_CONV `v`) THEN GEN_TAC THEN
+  EQ_TAC THEN Q.ID_SPEC_TAC `v` THEN Q.ID_SPEC_TAC `u` THEN
+  HO_MATCH_MP_TAC RTC_INDUCT THEN MESON_TAC [RTC_RULES, RTC_RTC]);
+
+val RTC_CASES1 = store_thm(
+  "RTC_CASES1",
+  ``!R (x:'a) y.  RTC R x y = (x = y) \/ ?u. R x u /\ RTC R u y``,
+  SIMP_TAC bool_ss [EQ_IMP_THM, FORALL_AND_THM] THEN CONJ_TAC THENL [
+    GEN_TAC THEN HO_MATCH_MP_TAC RTC_INDUCT THEN MESON_TAC [RTC_RULES],
+    MESON_TAC [RTC_RULES]
+  ]);
+
+val RTC_CASES2 = store_thm(
+  "RTC_CASES2",
+  ``!R (x:'a) y.  RTC R x y = (x = y) \/ ?u. RTC R x u /\ R u y``,
+  SIMP_TAC bool_ss [EQ_IMP_THM, FORALL_AND_THM] THEN CONJ_TAC THENL [
+    GEN_TAC THEN HO_MATCH_MP_TAC RTC_INDUCT THEN MESON_TAC [RTC_RULES],
+    MESON_TAC [RTC_RULES, RTC_SUBSET, RTC_RTC]
+  ]);
+
+val RTC_CASES_RTC_TWICE = store_thm(
+  "RTC_CASES_RTC_TWICE",
+  ``!R (x:'a) y. RTC R x y = ?u. RTC R x u /\ RTC R u y``,
+  SIMP_TAC bool_ss [EQ_IMP_THM, FORALL_AND_THM] THEN CONJ_TAC THENL [
+    GEN_TAC THEN HO_MATCH_MP_TAC RTC_INDUCT THEN MESON_TAC [RTC_RULES],
+    MESON_TAC [RTC_RULES, RTC_SUBSET, RTC_RTC]
+  ]);
+
+val TC_CASES1 =
 Q.store_thm
 ("TC_CASES1",
   `!R x z. TC R x z ==> R x z \/ ?y:'a. R x y /\ TC R y z`,
 GEN_TAC
- THEN TC_INDUCT_TAC 
+ THEN TC_INDUCT_TAC
  THEN MESON_TAC [REWRITE_RULE[transitive_def] TC_TRANSITIVE, TC_SUBSET]);
 
-val TC_CASES2 = 
+val TC_CASES2 =
 Q.store_thm
 ("TC_CASES2",
     `!R x z. TC R x z ==> R x z \/ ?y:'a. TC R x y /\ R y z`,
 GEN_TAC
- THEN TC_INDUCT_TAC 
+ THEN TC_INDUCT_TAC
  THEN MESON_TAC [REWRITE_RULE[transitive_def] TC_TRANSITIVE, TC_SUBSET]);
 
 
@@ -111,7 +270,7 @@ val NNF_TAC = CONV_TAC NNF_CONV;
  * Wellfoundedness: Every non-empty set has an R-minimal element.            *
  *---------------------------------------------------------------------------*)
 
-val WF_DEF = 
+val WF_DEF =
 Q.new_definition
  ("WF_DEF", `WF R = !B. (?w:'a. B w) ==> ?min. B min /\ !b. R b min ==> ~B b`);
 
@@ -130,9 +289,9 @@ Q.new_definition
  *                                                                           *
  *---------------------------------------------------------------------------*)
 
-val WF_INDUCTION_THM = 
+val WF_INDUCTION_THM =
 Q.store_thm("WF_INDUCTION_THM",
-`!(R:'a->'a->bool). 
+`!(R:'a->'a->bool).
    WF R ==> !P. (!x. (!y. R y x ==> P y) ==> P x) ==> !x. P x`,
 GEN_TAC THEN REWRITE_TAC[WF_DEF]
  THEN DISCH_THEN (fn th => GEN_TAC THEN (MP_TAC (Q.SPEC `\x:'a. ~P x` th)))
@@ -142,19 +301,19 @@ GEN_TAC THEN REWRITE_TAC[WF_DEF]
 
 
 val INDUCTION_WF_THM = Q.prove(
-`!R:'a->'a->bool. 
+`!R:'a->'a->bool.
      (!P. (!x. (!y. R y x ==> P y) ==> P x) ==> !x. P x) ==> WF R`,
-GEN_TAC THEN DISCH_TAC THEN REWRITE_TAC[WF_DEF] THEN GEN_TAC THEN 
- CONV_TAC CONTRAPOS_CONV THEN NNF_TAC THEN 
+GEN_TAC THEN DISCH_TAC THEN REWRITE_TAC[WF_DEF] THEN GEN_TAC THEN
+ CONV_TAC CONTRAPOS_CONV THEN NNF_TAC THEN
  DISCH_THEN (fn th => POP_ASSUM (MATCH_MP_TAC o BETA_RULE o Q.SPEC`\w. ~B w`)
-                      THEN ASSUME_TAC th) THEN GEN_TAC THEN 
+                      THEN ASSUME_TAC th) THEN GEN_TAC THEN
  CONV_TAC CONTRAPOS_CONV THEN NNF_TAC
  THEN POP_ASSUM MATCH_ACCEPT_TAC);
 
 
 (*---------------------------------------------------------------------------
- * A tactic for doing wellfounded induction. Lifted and adapted from 
- * John Harrison's definition of WO_INDUCT_TAC in the wellordering library. 
+ * A tactic for doing wellfounded induction. Lifted and adapted from
+ * John Harrison's definition of WO_INDUCT_TAC in the wellordering library.
  *---------------------------------------------------------------------------*)
 
 val _ = Parse.hide "C";
@@ -162,7 +321,7 @@ val _ = Parse.hide "C";
 val WF_INDUCT_TAC =
  let val wf_thm0 = CONV_RULE (ONCE_DEPTH_CONV ETA_CONV)
                    (REWRITE_RULE [TAUT`A==>B==>C = A/\B==>C`]
-                      (CONV_RULE (ONCE_DEPTH_CONV RIGHT_IMP_FORALL_CONV) 
+                      (CONV_RULE (ONCE_DEPTH_CONV RIGHT_IMP_FORALL_CONV)
                           WF_INDUCTION_THM))
       val [R,P] = fst(strip_forall(concl wf_thm0))
       val wf_thm1 = GENL [P,R](SPEC_ALL wf_thm0)
@@ -170,12 +329,12 @@ val WF_INDUCT_TAC =
     let val {Rator,Rand} = dest_comb w
         val {Name = "!",...} = dest_const Rator
         val thi = ISPEC Rand wf_thm1
-        val thf = CONV_RULE(ONCE_DEPTH_CONV 
+        val thf = CONV_RULE(ONCE_DEPTH_CONV
                             (BETA_CONV o assert (curry(op=) Rand o rator))) thi
     in MATCH_MP_TAC thf (asl,w)
     end
     handle _ => raise HOL_ERR{origin_structure = "<top-level>",
-                               origin_function = "WF_INDUCT_TAC", 
+                               origin_function = "WF_INDUCT_TAC",
                                       message = "Unanticipated term structure"}
  in tac
  end;
@@ -188,100 +347,100 @@ GEN_TAC THEN CONJ_TAC THEN Q.EXISTS_TAC`x` THEN REFL_TAC);
 val WF_NOT_REFL = Q.store_thm("WF_NOT_REFL",
 `!R x y. WF R ==> R x y ==> ~(x=y)`,
 REWRITE_TAC[WF_DEF]
-  THEN REPEAT GEN_TAC 
-  THEN DISCH_THEN (MP_TAC o Q.SPEC`\x. x=y`) 
-  THEN BETA_TAC THEN REWRITE_TAC[ex_lem] 
-  THEN STRIP_TAC 
-  THEN Q.UNDISCH_THEN `x=y` SUBST_ALL_TAC 
+  THEN REPEAT GEN_TAC
+  THEN DISCH_THEN (MP_TAC o Q.SPEC`\x. x=y`)
+  THEN BETA_TAC THEN REWRITE_TAC[ex_lem]
+  THEN STRIP_TAC
+  THEN Q.UNDISCH_THEN `x=y` SUBST_ALL_TAC
   THEN DISCH_TAC THEN RES_TAC);
 
 
 (*---------------------------------------------------------------------------
- * Some combinators for wellfounded relations. 
+ * Some combinators for wellfounded relations.
  *---------------------------------------------------------------------------*)
 
 (*---------------------------------------------------------------------------
  * The empty relation is wellfounded.
  *---------------------------------------------------------------------------*)
 
-val EMPTY_REL_DEF = 
+val EMPTY_REL_DEF =
 Q.new_definition
         ("EMPTY_REL_DEF", `EMPTY_REL (x:'a) (y:'a) = F`);
 
-val WF_Empty = 
+val WF_Empty =
 Q.store_thm
-  ("WF_EMPTY_REL", 
-   `WF (EMPTY_REL:'a->'a->bool)`, 
+  ("WF_EMPTY_REL",
+   `WF (EMPTY_REL:'a->'a->bool)`,
 REWRITE_TAC[EMPTY_REL_DEF,WF_DEF]);
 
 
 (*---------------------------------------------------------------------------
- * Subset: if R is a WF relation and P is a subrelation of R, then 
+ * Subset: if R is a WF relation and P is a subrelation of R, then
  * P is a wellfounded relation.
  *---------------------------------------------------------------------------*)
 
 val WF_SUBSET = Q.store_thm("WF_SUBSET",
-`!(R:'a->'a->bool) P. 
+`!(R:'a->'a->bool) P.
   WF R /\ (!x y. P x y ==> R x y) ==> WF P`,
-REWRITE_TAC[WF_DEF] 
- THEN REPEAT STRIP_TAC 
- THEN RES_TAC 
- THEN Q.EXISTS_TAC`min` 
- THEN ASM_REWRITE_TAC[] 
- THEN GEN_TAC 
- THEN DISCH_TAC 
+REWRITE_TAC[WF_DEF]
+ THEN REPEAT STRIP_TAC
+ THEN RES_TAC
+ THEN Q.EXISTS_TAC`min`
+ THEN ASM_REWRITE_TAC[]
+ THEN GEN_TAC
+ THEN DISCH_TAC
  THEN REPEAT RES_TAC);
 
 
 (*---------------------------------------------------------------------------
- * The transitive closure of a wellfounded relation is wellfounded. 
+ * The transitive closure of a wellfounded relation is wellfounded.
  * I got the clue about the witness from Peter Johnstone's book:
  * "Notes on Logic and Set Theory". An alternative proof that Bernhard
- * Schaetz showed me uses well-founded induction then case analysis. In that 
+ * Schaetz showed me uses well-founded induction then case analysis. In that
  * approach, the IH must be quantified over all sets, so that we can
  * specialize it later to an extension of B.
  *---------------------------------------------------------------------------*)
 
 val WF_TC = Q.store_thm("WF_TC",
 `!R:'a->'a->bool. WF R ==> WF(TC R)`,
-GEN_TAC THEN CONV_TAC CONTRAPOS_CONV THEN REWRITE_TAC[WF_DEF] 
+GEN_TAC THEN CONV_TAC CONTRAPOS_CONV THEN REWRITE_TAC[WF_DEF]
  THEN NNF_TAC THEN DISCH_THEN (Q.X_CHOOSE_THEN `B` MP_TAC)
- THEN DISCH_THEN (fn th => 
-       Q.EXISTS_TAC`\m:'a. ?a z. B a /\ TC R a m /\ TC R m z /\ B z` 
+ THEN DISCH_THEN (fn th =>
+       Q.EXISTS_TAC`\m:'a. ?a z. B a /\ TC R a m /\ TC R m z /\ B z`
        THEN BETA_TAC THEN CONJ_TAC THEN STRIP_ASSUME_TAC th)
  THENL
  [RES_TAC THEN RES_TAC THEN MAP_EVERY Q.EXISTS_TAC[`b`,  `b'`,  `w`]
    THEN ASM_REWRITE_TAC[],
   Q.X_GEN_TAC`m` THEN STRIP_TAC THEN Q.UNDISCH_TAC`TC R (a:'a) m`
-   THEN DISCH_THEN(fn th => STRIP_ASSUME_TAC 
+   THEN DISCH_THEN(fn th => STRIP_ASSUME_TAC
               (CONJ th (MATCH_MP TC_CASES2 th)))
    THENL
    [ Q.EXISTS_TAC`a` THEN ASM_REWRITE_TAC[] THEN RES_TAC
      THEN MAP_EVERY Q.EXISTS_TAC [`b'`, `z`] THEN ASM_REWRITE_TAC[],
-     Q.EXISTS_TAC`y` THEN ASM_REWRITE_TAC[] 
-     THEN MAP_EVERY Q.EXISTS_TAC[`a`,`z`] THEN ASM_REWRITE_TAC[] 
+     Q.EXISTS_TAC`y` THEN ASM_REWRITE_TAC[]
+     THEN MAP_EVERY Q.EXISTS_TAC[`a`,`z`] THEN ASM_REWRITE_TAC[]
      THEN IMP_RES_TAC TC_SUBSET]
-   THEN 
+   THEN
    IMP_RES_TAC(REWRITE_RULE[transitive_def] TC_TRANSITIVE)]);
 
 
 (*---------------------------------------------------------------------------
- * Inverse image theorem: mapping into a wellfounded relation gives a 
- * derived well founded relation. A "size" mapping, like "length" for 
+ * Inverse image theorem: mapping into a wellfounded relation gives a
+ * derived well founded relation. A "size" mapping, like "length" for
  * lists is such a relation.
  *
  * Proof.
  * f is total and maps from one n.e. set (Alpha) into another (Beta which is
- * "\y. ?x:'a. Alpha x /\ (f x = y)"). Since the latter is n.e. 
- * and has a wellfounded relation R on it, it has an R-minimal element 
- * (call it "min"). There exists an x:'a s.t. f x = min. Such an x is an 
- * R1-minimal element of Alpha (R1 is our derived ordering.) Why is x 
- * R1-minimal in Alpha? Well, if there was a y:'a s.t. R1 y x, then f y 
- * would not be in Beta (being less than f x, i.e., min). If f y wasn't in 
- * Beta, then y couldn't be in Alpha. 
+ * "\y. ?x:'a. Alpha x /\ (f x = y)"). Since the latter is n.e.
+ * and has a wellfounded relation R on it, it has an R-minimal element
+ * (call it "min"). There exists an x:'a s.t. f x = min. Such an x is an
+ * R1-minimal element of Alpha (R1 is our derived ordering.) Why is x
+ * R1-minimal in Alpha? Well, if there was a y:'a s.t. R1 y x, then f y
+ * would not be in Beta (being less than f x, i.e., min). If f y wasn't in
+ * Beta, then y couldn't be in Alpha.
  *---------------------------------------------------------------------------*)
 
-val inv_image_def = 
+val inv_image_def =
 Q.new_definition
 ("inv_image_def",
    `inv_image R (f:'a->'b) = \x y. R (f x) (f y):bool`);
@@ -289,43 +448,43 @@ Q.new_definition
 
 val WF_inv_image = Q.store_thm("WF_inv_image",
 `!R (f:'a->'b). WF R ==> WF (inv_image R f)`,
-REPEAT GEN_TAC 
+REPEAT GEN_TAC
   THEN REWRITE_TAC[inv_image_def,WF_DEF] THEN BETA_TAC
   THEN DISCH_THEN (fn th => Q.X_GEN_TAC`Alpha` THEN STRIP_TAC THEN MP_TAC th)
   THEN Q.SUBGOAL_THEN`?w:'b. (\y. ?x:'a. Alpha x /\ (f x = y)) w` MP_TAC
   THENL
-  [ BETA_TAC 
-     THEN MAP_EVERY Q.EXISTS_TAC[`f(w:'a)`,`w`] 
+  [ BETA_TAC
+     THEN MAP_EVERY Q.EXISTS_TAC[`f(w:'a)`,`w`]
      THEN ASM_REWRITE_TAC[],
-    DISCH_THEN (fn th => DISCH_THEN (MP_TAC o C MATCH_MP th)) THEN BETA_TAC 
-     THEN NNF_TAC 
+    DISCH_THEN (fn th => DISCH_THEN (MP_TAC o C MATCH_MP th)) THEN BETA_TAC
+     THEN NNF_TAC
      THEN REPEAT STRIP_TAC
      THEN Q.EXISTS_TAC`x`
      THEN ASM_REWRITE_TAC[]
-     THEN GEN_TAC 
+     THEN GEN_TAC
      THEN DISCH_THEN (ANTE_RES_THEN (MP_TAC o Q.SPEC`b`))
      THEN REWRITE_TAC[]]);
 
 
 (*---------------------------------------------------------------------------
  * Now the WF recursion theorem. Based on Tobias Nipkow's Isabelle development
- * of wellfounded recursion, which itself is a generalization of Mike 
+ * of wellfounded recursion, which itself is a generalization of Mike
  * Gordon's HOL development of the primitive recursion theorem.
  *---------------------------------------------------------------------------*)
 
-val RESTRICT_DEF = 
+val RESTRICT_DEF =
 Q.new_definition
 ("RESTRICT_DEF",
    `RESTRICT (f:'a->'b) R (x:'a) = \y:'a. if R y x then f y else ARB`);
 
 
 (*---------------------------------------------------------------------------
- * Obvious, but crucially useful. Unary case. Handling the n-ary case might 
+ * Obvious, but crucially useful. Unary case. Handling the n-ary case might
  * be messy!
  *---------------------------------------------------------------------------*)
 
 val RESTRICT_LEMMA = Q.store_thm("RESTRICT_LEMMA",
-`!(f:'a->'b) R (y:'a) (z:'a).   
+`!(f:'a->'b) R (y:'a) (z:'a).
     R y z ==> (RESTRICT f R z y = f y)`,
 REWRITE_TAC [RESTRICT_DEF] THEN BETA_TAC THEN REPEAT GEN_TAC THEN STRIP_TAC
 THEN ASM_REWRITE_TAC[]);
@@ -337,43 +496,43 @@ THEN ASM_REWRITE_TAC[]);
  *---------------------------------------------------------------------------*)
 
 val CUTS_EQ = Q.prove(
-`!R f g (x:'a). 
-   (RESTRICT f R x = RESTRICT g R x) 
+`!R f g (x:'a).
+   (RESTRICT f R x = RESTRICT g R x)
     = !y:'a. R y x ==> (f y:'b = g y)`,
 REPEAT GEN_TAC THEN REWRITE_TAC[RESTRICT_DEF]
  THEN CONV_TAC (DEPTH_CONV FUN_EQ_CONV) THEN BETA_TAC THEN EQ_TAC
  THENL
- [ CONV_TAC RIGHT_IMP_FORALL_CONV THEN GEN_TAC 
+ [ CONV_TAC RIGHT_IMP_FORALL_CONV THEN GEN_TAC
    THEN DISCH_THEN (MP_TAC o Q.SPEC`y`) THEN COND_CASES_TAC THEN REWRITE_TAC[],
-   DISCH_TAC THEN GEN_TAC THEN COND_CASES_TAC THEN RES_TAC 
+   DISCH_TAC THEN GEN_TAC THEN COND_CASES_TAC THEN RES_TAC
    THEN ASM_REWRITE_TAC[]]);
 
 
-val EXPOSE_CUTS_TAC = 
-   BETA_TAC THEN AP_THM_TAC THEN AP_TERM_TAC 
-     THEN REWRITE_TAC[CUTS_EQ] 
+val EXPOSE_CUTS_TAC =
+   BETA_TAC THEN AP_THM_TAC THEN AP_TERM_TAC
+     THEN REWRITE_TAC[CUTS_EQ]
      THEN REPEAT STRIP_TAC;
 
 
 (*---------------------------------------------------------------------------
- * The set of approximations to the function being defined, restricted to 
+ * The set of approximations to the function being defined, restricted to
  * being R-parents of x. This has the consequence (approx_ext):
  *
  *    approx R M x f = !w. f w = ((R w x) => (M (RESTRICT f R w w) | (@v. T))
  *
  *---------------------------------------------------------------------------*)
 
-val approx_def = 
+val approx_def =
 Q.new_definition
   ("approx_def",
    `approx R M x (f:'a->'b) = (f = RESTRICT (\y. M (RESTRICT f R y) y) R x)`);
 
 (* This could, in fact, be the definition. *)
-val approx_ext = 
+val approx_ext =
 BETA_RULE(ONCE_REWRITE_RULE[RESTRICT_DEF]
     (CONV_RULE (ONCE_DEPTH_CONV (Q.X_FUN_EQ_CONV`w`)) approx_def));
 
-val approx_SELECT0 = 
+val approx_SELECT0 =
   Q.GEN`g` (Q.SPEC`g`
      (BETA_RULE(Q.ISPEC `\f:'a->'b. approx R M x f` boolTheory.SELECT_AX)));
 
@@ -381,7 +540,7 @@ val approx_SELECT1 = CONV_RULE FORALL_IMP_CONV  approx_SELECT0;
 
 
 (*---------------------------------------------------------------------------
- * Choose an approximation for R and M at x. Thus it is a 
+ * Choose an approximation for R and M at x. Thus it is a
  * kind of "lookup" function, associating partial functions with arguments.
  * One can easily prove
  *  (?g. approx R M x g) ==>
@@ -389,7 +548,7 @@ val approx_SELECT1 = CONV_RULE FORALL_IMP_CONV  approx_SELECT0;
  *                                    |  (@v. T)))
  *---------------------------------------------------------------------------*)
 
-val the_fun_def = 
+val the_fun_def =
 Q.new_definition
 ("the_fun_def",
   `the_fun R M x = @f:'a->'b. approx R M x f`);
@@ -400,21 +559,21 @@ val approx_the_fun2 = SUBS [Q.SPECL[`R`,`M`,`x`,`the_fun R M x`] approx_ext]
                            approx_the_fun1;
 
 val the_fun_rw1 = Q.prove(
- `(?g:'a->'b. approx R M x g) 
-      ==> 
-  !w. R w x 
-       ==> 
+ `(?g:'a->'b. approx R M x g)
+      ==>
+  !w. R w x
+       ==>
      (the_fun R M x w = M (RESTRICT (the_fun R M x) R w) w)`,
  DISCH_THEN (MP_TAC o MP approx_the_fun2) THEN
- DISCH_THEN (fn th => GEN_TAC THEN MP_TAC (SPEC_ALL th)) 
- THEN COND_CASES_TAC 
+ DISCH_THEN (fn th => GEN_TAC THEN MP_TAC (SPEC_ALL th))
+ THEN COND_CASES_TAC
  THEN ASM_REWRITE_TAC[]);
 
 val the_fun_rw2 = Q.prove(
  `(?g:'a->'b. approx R M x g)  ==> !w. ~R w x ==> (the_fun R M x w = ARB)`,
 DISCH_THEN (MP_TAC o MP approx_the_fun2) THEN
- DISCH_THEN (fn th => GEN_TAC THEN MP_TAC (SPEC_ALL th)) 
- THEN COND_CASES_TAC 
+ DISCH_THEN (fn th => GEN_TAC THEN MP_TAC (SPEC_ALL th))
+ THEN COND_CASES_TAC
  THEN ASM_REWRITE_TAC[]);
 
 (*---------------------------------------------------------------------------
@@ -425,15 +584,15 @@ DISCH_THEN (MP_TAC o MP approx_the_fun2) THEN
  *
  * as the function made available for M to use, along with x. Notice that the
  * function unrolls properly for each R-ancestor, but only gets applied
- * "parentwise", i.e., you can't apply it to any old ancestor, just to a 
+ * "parentwise", i.e., you can't apply it to any old ancestor, just to a
  * parent. This holds recursively, which is what the theorem we eventually
  * prove is all about.
  *---------------------------------------------------------------------------*)
 
-val WFREC_DEF = 
+val WFREC_DEF =
 Q.new_definition
 ("WFREC_DEF",
-  `WFREC R (M:('a->'b) -> ('a->'b)) = 
+  `WFREC R (M:('a->'b) -> ('a->'b)) =
      \x. M (RESTRICT (the_fun (TC R) (\f v. M (RESTRICT f R v) v) x) R x) x`);
 
 
@@ -442,13 +601,13 @@ Q.new_definition
  *---------------------------------------------------------------------------*)
 
 val APPROX_EQUAL_BELOW = Q.prove(
-`!R M f g u v. 
+`!R M f g u v.
   WF R /\ transitive R /\
-  approx R M u f /\ approx R M v g 
-  ==> !x:'a. R x u ==> R x v 
+  approx R M u f /\ approx R M v g
+  ==> !x:'a. R x u ==> R x v
              ==> (f x:'b = g x)`,
 REWRITE_TAC[approx_ext] THEN REPEAT GEN_TAC THEN STRIP_TAC
-  THEN WF_INDUCT_TAC THEN Q.EXISTS_TAC`R` 
+  THEN WF_INDUCT_TAC THEN Q.EXISTS_TAC`R`
   THEN ASM_REWRITE_TAC[] THEN REPEAT STRIP_TAC
   THEN REPEAT COND_CASES_TAC THEN RES_TAC
   THEN EXPOSE_CUTS_TAC
@@ -458,7 +617,7 @@ REWRITE_TAC[approx_ext] THEN REPEAT GEN_TAC THEN STRIP_TAC
   THEN FIRST_ASSUM MATCH_MP_TAC
   THEN RES_TAC THEN ASM_REWRITE_TAC[]);
 
-val AGREE_BELOW = 
+val AGREE_BELOW =
    REWRITE_RULE[TAUT`A==>B==>C==>D = B/\C/\A==>D`]
     (CONV_RULE (DEPTH_CONV RIGHT_IMP_FORALL_CONV) APPROX_EQUAL_BELOW);
 
@@ -476,12 +635,12 @@ val RESTRICT_FUN_EQ = Q.prove(
      R v u
      ==> (RESTRICT f R v = g)`,
 REWRITE_TAC[RESTRICT_DEF,transitive_def] THEN REPEAT STRIP_TAC
-  THEN CONV_TAC (Q.X_FUN_EQ_CONV`w`) THEN BETA_TAC THEN GEN_TAC 
+  THEN CONV_TAC (Q.X_FUN_EQ_CONV`w`) THEN BETA_TAC THEN GEN_TAC
   THEN COND_CASES_TAC (* on R w v *)
-  THENL [ MATCH_MP_TAC AGREE_BELOW THEN REPEAT Q.ID_EX_TAC 
+  THENL [ MATCH_MP_TAC AGREE_BELOW THEN REPEAT Q.ID_EX_TAC
             THEN RES_TAC THEN ASM_REWRITE_TAC[transitive_def],
-          Q.UNDISCH_TAC`approx R M v (g:'a->'b)` 
-            THEN DISCH_THEN(fn th => 
+          Q.UNDISCH_TAC`approx R M v (g:'a->'b)`
+            THEN DISCH_THEN(fn th =>
                    ASM_REWRITE_TAC[REWRITE_RULE[approx_ext]th])]);
 
 
@@ -492,46 +651,46 @@ REWRITE_TAC[RESTRICT_DEF,transitive_def] THEN REPEAT STRIP_TAC
 val EXISTS_LEMMA = Q.prove(
 `!R M. WF R /\ transitive R ==> !x. ?f:'a->'b. approx R M x f`,
 REPEAT GEN_TAC THEN STRIP_TAC
-  THEN WF_INDUCT_TAC 
+  THEN WF_INDUCT_TAC
   THEN Q.EXISTS_TAC`R` THEN ASM_REWRITE_TAC[] THEN GEN_TAC
   THEN DISCH_THEN  (* Adjust IH by applying Choice *)
-    (ASSUME_TAC o Q.GEN`y` o Q.DISCH`R (y:'a) (x:'a)` 
+    (ASSUME_TAC o Q.GEN`y` o Q.DISCH`R (y:'a) (x:'a)`
                 o (fn th => REWRITE_RULE[GSYM the_fun_def] th)
                 o SELECT_RULE o UNDISCH o Q.ID_SPEC)
   THEN Q.EXISTS_TAC`\p. R p x => M (the_fun R M p) p | ARB` (* witness *)
-  THEN REWRITE_TAC[approx_ext] THEN BETA_TAC THEN GEN_TAC 
+  THEN REWRITE_TAC[approx_ext] THEN BETA_TAC THEN GEN_TAC
   THEN COND_CASES_TAC
   THEN ASM_REWRITE_TAC[boolTheory.ARB_DEF]
   THEN EXPOSE_CUTS_TAC
   THEN RES_THEN (SUBST1_TAC o REWRITE_RULE[approx_def])     (* use IH *)
-  THEN REWRITE_TAC[CUTS_EQ] 
+  THEN REWRITE_TAC[CUTS_EQ]
   THEN Q.X_GEN_TAC`v` THEN BETA_TAC THEN DISCH_TAC
-  THEN RULE_ASSUM_TAC(REWRITE_RULE[transitive_def]) THEN RES_TAC 
+  THEN RULE_ASSUM_TAC(REWRITE_RULE[transitive_def]) THEN RES_TAC
   THEN ASM_REWRITE_TAC[]
   THEN EXPOSE_CUTS_TAC
   THEN MATCH_MP_TAC RESTRICT_FUN_EQ
-  THEN MAP_EVERY Q.EXISTS_TAC[`M`,`w`] 
+  THEN MAP_EVERY Q.EXISTS_TAC[`M`,`w`]
   THEN ASM_REWRITE_TAC[transitive_def]
   THEN RES_TAC);
 
- 
+
 val the_fun_unroll = Q.prove(
  `!R M x (w:'a).
-     WF R /\ transitive R 
-       ==> R w x 
+     WF R /\ transitive R
+       ==> R w x
         ==> (the_fun R M x w:'b = M (RESTRICT (the_fun R M x) R w) w)`,
-REPEAT GEN_TAC THEN DISCH_TAC 
+REPEAT GEN_TAC THEN DISCH_TAC
   THEN Q.ID_SPEC_TAC`w`
-  THEN MATCH_MP_TAC the_fun_rw1 
+  THEN MATCH_MP_TAC the_fun_rw1
   THEN MATCH_MP_TAC EXISTS_LEMMA
   THEN POP_ASSUM ACCEPT_TAC);
 
 (*---------------------------------------------------------------------------
  * Unrolling works for any R M and x, hence it works for "TC R" and
- * "\f v. M (f % R,v) v". 
+ * "\f v. M (f % R,v) v".
  *---------------------------------------------------------------------------*)
 
-val the_fun_TC0 = 
+val the_fun_TC0 =
   BETA_RULE
    (REWRITE_RULE[MATCH_MP WF_TC (Q.ASSUME`WF (R:'a->'a->bool)`),
                  TC_TRANSITIVE]
@@ -543,12 +702,12 @@ val the_fun_TC0 =
  *---------------------------------------------------------------------------*)
 val TC_RESTRICT_LEMMA = Q.prove(
  `!(f:'a->'b) R w. RESTRICT (RESTRICT f (TC R) w) R w = RESTRICT f R w`,
-REPEAT GEN_TAC 
+REPEAT GEN_TAC
   THEN REWRITE_TAC[RESTRICT_DEF]
-  THEN CONV_TAC (Q.X_FUN_EQ_CONV`p`) 
-  THEN BETA_TAC THEN GEN_TAC 
+  THEN CONV_TAC (Q.X_FUN_EQ_CONV`p`)
+  THEN BETA_TAC THEN GEN_TAC
   THEN COND_CASES_TAC
-  THENL [IMP_RES_TAC TC_SUBSET, ALL_TAC] 
+  THENL [IMP_RES_TAC TC_SUBSET, ALL_TAC]
   THEN ASM_REWRITE_TAC[]);
 
 val the_fun_TC = REWRITE_RULE[TC_RESTRICT_LEMMA] the_fun_TC0;
@@ -560,21 +719,21 @@ val the_fun_TC = REWRITE_RULE[TC_RESTRICT_LEMMA] the_fun_TC0;
 
 val WFREC_THM = Q.store_thm
 ("WFREC_THM",
-  `!R. !M:('a -> 'b) -> ('a -> 'b). 
+  `!R. !M:('a -> 'b) -> ('a -> 'b).
       WF R ==> !x. WFREC R M x = M (RESTRICT (WFREC R M) R x) x`,
-REPEAT STRIP_TAC THEN REWRITE_TAC[WFREC_DEF] 
+REPEAT STRIP_TAC THEN REWRITE_TAC[WFREC_DEF]
   THEN EXPOSE_CUTS_TAC THEN BETA_TAC
-  THEN IMP_RES_TAC TC_SUBSET 
+  THEN IMP_RES_TAC TC_SUBSET
   THEN USE_TAC the_fun_TC
   THEN EXPOSE_CUTS_TAC
   THEN MATCH_MP_TAC AGREE_BELOW
   THEN MAP_EVERY Q.EXISTS_TAC [`TC R`, `\f v. M (RESTRICT f R v) v`, `x`, `y`]
-  THEN IMP_RES_TAC WF_TC 
+  THEN IMP_RES_TAC WF_TC
   THEN ASSUME_TAC(SPEC_ALL TC_TRANSITIVE)
   THEN IMP_RES_TAC TC_SUBSET THEN POP_ASSUM (K ALL_TAC)
-  THEN ASM_REWRITE_TAC[] 
+  THEN ASM_REWRITE_TAC[]
   THEN REPEAT CONJ_TAC
-  THENL [ RULE_ASSUM_TAC(REWRITE_RULE[transitive_def]) THEN RES_TAC, 
+  THENL [ RULE_ASSUM_TAC(REWRITE_RULE[transitive_def]) THEN RES_TAC,
           ALL_TAC,ALL_TAC]
   THEN MATCH_MP_TAC approx_the_fun1
   THEN MATCH_MP_TAC EXISTS_LEMMA
@@ -585,9 +744,9 @@ REPEAT STRIP_TAC THEN REWRITE_TAC[WFREC_DEF]
  * This is what is used by TFL.                                              *
  *---------------------------------------------------------------------------*)
 
-val WFREC_COROLLARY = 
+val WFREC_COROLLARY =
  Q.store_thm("WFREC_COROLLARY",
-  `!M R (f:'a->'b). 
+  `!M R (f:'a->'b).
         (f = WFREC R M) ==> WF R ==> !x. f x = M (RESTRICT f R x) x`,
 REPEAT GEN_TAC THEN DISCH_TAC THEN ASM_REWRITE_TAC[WFREC_THM]);
 
@@ -598,14 +757,14 @@ REPEAT GEN_TAC THEN DISCH_TAC THEN ASM_REWRITE_TAC[WFREC_THM]);
 
 val WF_RECURSION_THM = Q.store_thm("WF_RECURSION_THM",
 `!R. WF R ==> !M. ?!f:'a->'b. !x. f x = M (RESTRICT f R x) x`,
-GEN_TAC THEN DISCH_TAC THEN GEN_TAC THEN CONV_TAC EXISTS_UNIQUE_CONV 
+GEN_TAC THEN DISCH_TAC THEN GEN_TAC THEN CONV_TAC EXISTS_UNIQUE_CONV
 THEN CONJ_TAC THENL
 [Q.EXISTS_TAC`WFREC R M` THEN MATCH_MP_TAC WFREC_THM THEN POP_ASSUM ACCEPT_TAC,
  REPEAT STRIP_TAC THEN CONV_TAC (Q.X_FUN_EQ_CONV`w`) THEN WF_INDUCT_TAC
  THEN Q.EXISTS_TAC`R` THEN CONJ_TAC THENL
- [ FIRST_ASSUM ACCEPT_TAC, 
-   GEN_TAC THEN DISCH_TAC THEN ASM_REWRITE_TAC[] THEN AP_THM_TAC THEN 
-   AP_TERM_TAC THEN REWRITE_TAC[CUTS_EQ] THEN GEN_TAC THEN 
+ [ FIRST_ASSUM ACCEPT_TAC,
+   GEN_TAC THEN DISCH_TAC THEN ASM_REWRITE_TAC[] THEN AP_THM_TAC THEN
+   AP_TERM_TAC THEN REWRITE_TAC[CUTS_EQ] THEN GEN_TAC THEN
    FIRST_ASSUM MATCH_ACCEPT_TAC]]);
 
 
